
\section{Mathematical Formulations}

\subsection{Ensemble Learning Methods}

\subsubsection{Bagging}
Bagging (Bootstrap Aggregating) combines predictions from multiple models trained on different bootstrap samples:
\begin{equation}
\hat{f}_{bag}(x) = \frac{1}{B} \sum_{b=1}^{B} \hat{f}_b(x)
\end{equation}
where $B$ is the number of bootstrap samples and $\hat{f}_b(x)$ is the prediction from the $b$-th model.

\subsubsection{Voting}
Weighted voting combines predictions using predetermined weights:
\begin{equation}
\hat{f}_{vote}(x) = \sum_{i=1}^{M} w_i \hat{f}_i(x), \quad \sum_{i=1}^{M} w_i = 1
\end{equation}
where $w_i$ is the weight assigned to the $i$-th model and $M$ is the total number of models.

\subsubsection{Stacking}
Stacking uses a meta-learner to combine base model predictions:
\begin{equation}
\hat{f}_{stack}(x) = g(\hat{f}_1(x), \hat{f}_2(x), ..., \hat{f}_M(x))
\end{equation}
where $g(\cdot)$ is the meta-learner function.

\subsection{Base Learning Algorithms}

\subsubsection{Linear Regression}
\begin{equation}
\hat{y} = \beta_0 + \sum_{j=1}^{p} \beta_j x_j
\end{equation}

\subsubsection{Ridge Regression}
\begin{equation}
\hat{\beta}_{ridge} = \arg\min_{\beta} \left\{ \sum_{i=1}^{n} (y_i - x_i^T\beta)^2 + \lambda \sum_{j=1}^{p} \beta_j^2 \right\}
\end{equation}

\subsubsection{K-Nearest Neighbors}
\begin{equation}
\hat{f}(x) = \frac{1}{k} \sum_{x_i \in N_k(x)} y_i
\end{equation}
where $N_k(x)$ represents the $k$ nearest neighbors of $x$.

\subsubsection{Neural Network}
\begin{equation}
f(x) = \sigma\left( \sum_{j=1}^{H} w_j^{(2)} \sigma\left( \sum_{i=1}^{D} w_{ij}^{(1)} x_i + b_j^{(1)} \right) + b^{(2)} \right)
\end{equation}

\subsubsection{Support Vector Regression}
\begin{equation}
f(x) = \sum_{i=1}^{n} (\alpha_i - \alpha_i^*) K(x_i, x) + b
\end{equation}

\subsection{Evaluation Metrics}

\subsubsection{Root Mean Square Error}
\begin{equation}
RMSE = \sqrt{\frac{1}{n} \sum_{i=1}^{n} (y_i - \hat{y}_i)^2}
\end{equation}

\subsubsection{Coefficient of Determination}
\begin{equation}
R^2 = 1 - \frac{\sum_{i=1}^{n} (y_i - \hat{y}_i)^2}{\sum_{i=1}^{n} (y_i - \bar{y})^2}
\end{equation}
